## 公理系统的推理过程

### 例题

- 定理1，P→¬¬P

证明：

<table style="border-collapse:collapse">
<tr>
<td>1. (P→¬Q)→(Q→¬P) </td>
<td>公理14</td>
</tr>
<tr>
<td>2. (¬P→¬P)→(P→¬¬P) </td>
<td> P用¬P，Q用P代入 </td>
</tr>
<tr>
<td>3. P→P </td>
<td>公理1</td>
</tr>
<tr>
<td>4. ¬P→¬P </td>
<td>P用¬P代入</td>
</tr>
<tr>
<td>5. P→¬¬P </td>
<td>三段论，分离2，4</td>
</tr>
</table>

- 定理2，(P→Q)→((R→P)→(R→Q))

证明：

<table style="border-collapse: collapse;">
<tr>
<td> (P→Q)→((Q→R)→(P→R)) </td>
<td>公理3</td>
</tr>
<tr>
<td> (R→P)→((P→Q)→(R→Q)) </td>
<td>P用R，Q用P，R用Q</td>
</tr>
<tr>
<td> (P→(Q→R))→(Q→(P→R)) </td>
<td>公理2</td>
</tr>
<tr>
<td>((R→P)→((P→Q)→(R→Q)))→((P→Q)→((R→P)→(R→Q)))</td>
<td>P用R→P，Q用P→Q，R用R→Q代入</td>
</tr>
<tr>
<td>(P→Q)→((R→P)→(R→Q))</td>
<td>三段论，分离2，4</td>
</tr>	
</table>

- 定理3：(P→Q)→(¬Q→¬P)

证明：

<table style="border-collapse: collapse;">
<tr>
<td>1. P→¬¬P</td>
<td>定理1</td>
</tr>
<tr>
<td>2. Q→¬¬Q</td>
<td>P用Q代入</td>
</tr>
<tr>
<td>3. (P→¬Q)→(Q→¬P)</td>
<td>公理14</td>
</tr>
<tr>
<td>4. (P→¬¬Q)→(¬Q→¬P)</td>
<td>Q用¬Q代入</td>
</tr>
<tr>
<td>5. (P→Q)→((P→Q)→(P→¬¬Q))</td>
<td>定理2</td>
</tr>	
<tr>
<td>6. (Q→¬¬Q)→((P→Q)→(P→¬¬Q))</td>
<td>P用Q，Q用¬¬Q，R用P代入</td>
</tr>	
<tr>
<td>7. (P→Q)→(P→¬¬Q)</td>
<td>三段论，分离6，2</td>
</tr>
<tr>
<td>(P→Q)→((Q→R)→(P→R))</td>
<td>公理3</td>
</tr>
<tr>
<td>((P→Q)→(P→¬¬Q))→(((P→¬¬Q)→(¬Q→¬P))→((P→Q)→(¬Q→¬P)))</td>
<td>P用P→Q，Q用P→¬¬Q，R用¬Q→¬P</td>
</tr>
<tr>
<td>((P→¬¬Q)→(¬Q→¬P))→((P→Q)→(¬Q→¬P))</td>
<td>三段论，9，7分离</td>
</tr>
<tr>
<td>(P→Q)→(¬Q→¬P)</td>
<td>三段论，10，4分离</td>
</tr>
</table>

- 定理4：P→((P→Q)→Q)

<table style="border-collapse: collapse;">
<tr>
<td>P→P</td>
<td>公理1</td>
</tr>
<tr>
<td>(P→Q)→(P→Q)</td>
<td>P用P→Q代入</td>
</tr>
<tr>
<td>(P→(Q→R))→(Q→(P→R))</td>
<td>公理2</td>
</tr>
<tr>
<td>(P→(P→Q))→(P→((P→Q)→Q))</td>
<td>P用P→Q，Q用P，R用Q代入</td>
</tr>
<tr>
<td>P→((P→Q)→Q)</td>
<td>三段论，分离4，2</td>
</tr>
</table>

已知公理：

- A: P→(Q→P)
- B: (P→(Q→R))→((P→Q)→(P→R))
- C: (P→(Q→P))→(Q→(P→R))
- D: P→(P∨Q)
- E: (P∨Q)→(Q∨P)

及分离规则和代入规则， 证明公式(R∧¬R)∨(P→P)

<table style="border-collapse: collapse;">
<tr>
<td>1. P→(Q→P)</td>
<td>公理A</td>
</tr>
<tr>
<td>2. (P→(Q→R))→((P→Q)→(P→R))</td>
<td>公理B</td>
</tr>
<tr>
<td>3. (P→(Q→P))→((P→Q)→(P→P))</td>
<td>R用P代入</td>
</tr>
<tr>
<td>4. (P→Q)→(P→P)</td>
<td>三段论，3，1分离</td>
</tr>
<tr>
<td>5. (P→(Q→P))→(P→P)</td>
<td>Q用Q→P来代替</td>
</tr>
<tr>
<td>6. P→P</td>
<td>三段论，1，5分离</td>
</tr>
<tr>
<td>7. P→(P∨Q)</td>
<td>公理D</td>
</tr>
<tr>
<td>8. (P→P)→((P→P)∨(R∧¬R))</td>
<td>P用P→P，Q用R∧¬R代入</td>
</tr>
<tr>
<td>9. (P→P)∨(R∧¬R)</td>
<td>三段论，8，6分离</td>
</tr>
<td>10. (P∨Q)→(Q∨P)</td>
<td>公理E</td>
</tr>
</tr>
<td>11. ((P→P)∨(R∧¬R))→((R∧¬R)∨(P→P))</td>
<td>P用P→P，Q用R∧¬R代入</td>
</tr>
<tr>
<td>12. (R∧¬R)∨(P→P)</td>
<td>三段论，分离 11，9</td>
</tr>
</table>